theories/named_props.v
@@ -1,0 +1,378 @@
+(* vendored from https://github.com/tchajed/iris-named-props *)
+From iris.proofmode Require Import string_ident.
+From iris.proofmode Require Import tactics environments intro_patterns monpred.
+
+Set Default Proof Using "Type".
+
+(* NamedProps implements [name ∷ P], which is equivalent to P but knows to
+   name itself [name] when destructed. The syntax is intended to be analogous
+   to in Gallina where you might write [forall (Hfoo: 3 < 4), ...] for a
+   hypothesis that would be introduced as [Hfoo] using automatic names.
+
+  To use this library, write your definitions with [name ∷ P] for each conjunct.
+  Then, use [iNamed "H"] to destruct an invariant "H" into its conjuncts, using
+  their specified names. [iNamed] also introduces existentials with the names
+  for the Coq binders.
+
+  The names in a named proposition are not actually names but full-blown Iris intro
+  patterns. This means you can write [#H] to automatically introduce to the
+  persistent context, [%H] to name a pure fact (using string_to_ident), or even
+  something crazy like ["[<- H]"] to destruct the hypothesis and rewrite by the
+  first conjunct.
+
+  There are a several top-level tactics provided to work with named
+  propositions:
+  - [iNamed "H"] names a single hypothesis. This is the most common usage.
+  - [iNamed 1] on a wand introduces and destructs the premise.
+  - [iNamed] names any anonymous hypotheses (without destructing them).
+  - [iNamedAccu] is like [iAccu] - it solves a goal which is an evar with the
+    conjunction of all the hypotheses - but produces a conjunction of named
+    hypotheses. This is especially useful when that evar ?Q shows up as a
+    premise in a wand, [?Q -∗ ...], at which point you can do [iNamed 1] to
+    restore the context, including all the names.
+  - [iFrameNamed] is a work-in-progress tactic to frame a goal with named
+    conjuncts with the hypotheses using the names. This is intended to be much
+    faster than framing the entire persistent and spatial contexts.
+
+  Note that this library provides general support for propositions and is not
+  specific to definitions. You can use named hypotheses in Hoare logic
+  preconditions (to make the first iIntros more stable), in the postcondition
+  (to make it easier for the caller to re-introduce hypotheses), or in loop
+  invariants (to serve both of these purposes). If they ever get in the way you
+  can always [rewrite /named] to get rid of the names.
+ *)
+
+(* Named props are defined to be the underlying prop. We used to have this
+sealed, but it turns out that this inconveniently required many forwarding
+typeclass instances (for things like [IntoPure], [Persistent], and framing) and
+we didn't run into any issues making it completely transparent.
+
+For efficiency reasons, we don't have [(PROP:bi) (P:PROP)], since this requires
+a coercion to the carrier of [PROP]. *)
+Definition named {A} (name: string) (P: A): A := P.
+
+Section named.
+  Context {PROP:bi}.
+
+  Theorem to_named name (P: PROP) : P -∗ named name P.
+  Proof. auto. Qed.
+  Theorem from_named name (P: PROP) : named name P -∗ P.
+  Proof. auto. Qed.
+
+  (* Implementation of [iNamedAccu]; the soundness proof basically shows these
+  definitions are equivalent to the ones used in the [iAccu] implementation,
+  since we can simply unfold [named]. *)
+
+  Fixpoint env_to_named_prop_go (acc : PROP) (Γ : env PROP) : PROP :=
+    match Γ with
+    | Enil => acc
+    | Esnoc Γ (INamed name) P => env_to_named_prop_go (named name P ∗ acc)%I Γ
+    | Esnoc Γ _ P => env_to_named_prop_go (named "?" P ∗ acc)%I Γ
+    end.
+  Definition env_to_named_prop (Γ : env PROP) : PROP :=
+    match Γ with
+    | Enil => emp%I
+    | Esnoc Γ (INamed name) P => env_to_named_prop_go (named name P) Γ
+    | Esnoc Γ _ P => env_to_named_prop_go (named "?" P) Γ
+    end.
+
+  Theorem env_to_named_prop_go_unname (acc: PROP) Γ :
+    env_to_named_prop_go acc Γ = env_to_prop_go acc Γ.
+  Proof.
+    revert acc.
+    induction Γ; simpl; auto; intros.
+    rewrite IHΓ.
+    destruct i; simpl; auto.
+  Qed.
+
+  Theorem env_to_named_prop_unname (Γ: env PROP) :
+    env_to_named_prop Γ = env_to_prop Γ.
+  Proof.
+    destruct Γ; auto.
+    destruct i; simpl; rewrite env_to_named_prop_go_unname //.
+  Qed.
+
+  Theorem env_to_named_prop_sound (Γ: env PROP) :
+    env_to_named_prop Γ ≡ ([∗] Γ)%I.
+  Proof.
+    rewrite env_to_named_prop_unname env_to_prop_sound //.
+  Qed.
+
+  Lemma tac_named_accu Δ (P: PROP) :
+    env_to_named_prop (env_spatial Δ) = P →
+    envs_entails Δ P.
+  Proof.
+    rewrite env_to_named_prop_unname.
+    apply coq_tactics.tac_accu.
+  Qed.
+
+  Lemma tac_delay_split (R P Q: PROP) :
+    (P ∗ R) -∗ (R -∗ Q) -∗ P ∗ Q.
+  Proof.
+    iIntros "[$ R] Hwand".
+    iApply ("Hwand" with "R").
+  Qed.
+
+End named.
+
+Ltac to_pm_ident H :=
+  lazymatch type of H with
+  | string => constr:(INamed H)
+  | ident => constr:(H)
+  end.
+
+Local Ltac iDeex_as i x :=
+  let x' := fresh x in
+  iDestructHyp i as (x') i.
+
+Ltac iDeex :=
+  repeat match goal with
+         | |- context[Esnoc _ ?i (bi_exist (fun x => _))] =>
+           iDeex_as i x
+         end.
+
+(** [IsExistential] identifies propositions that should be destructed as
+existentials by [iDeex]. *)
+Class IsExistential {PROP:bi} (P: PROP) := is_existential {}.
+Global Arguments is_existential {PROP P} : assert.
+Global Instance is_existential_exist {PROP:bi} {A} (Φ: A → PROP) :
+  IsExistential (bi_exist Φ).
+Proof. Qed.
+
+(** [IsSplittable] identifies separating conjunction-like propositions that
+should be split by [iNamed] as it traverses a proposition for named conjuncts.
+*)
+Class IsSplittable {PROP:bi} (P: PROP) := is_splittable {}.
+Global Arguments IsSplittable {_} _%I : assert.
+Global Arguments is_splittable {PROP P} : assert.
+Global Instance is_splittable_sep {PROP:bi} (P Q: PROP) :
+  IsSplittable (P ∗ Q).
+Proof. Qed.
+
+Lemma make_monPred_at_named {I : biIndex} {PROP : bi} name (i : I) (P : monPred I PROP) (𝓟 : PROP) :
+  MakeMonPredAt i P 𝓟 →
+  MakeMonPredAt i (named name P) (named name 𝓟).
+Proof. done. Qed.
+
+(* This is not an instance since Coq would try and apply the instance at every
+step in the type class resolution since [named name P] unfolds to just [P].
+Instead we register a hint that only applies when the goal contains [named]. *)
+Global Hint Extern 0 (MakeMonPredAt _ (named _ _) _) => apply make_monPred_at_named : typeclass_instances.
+
+(** tc_is_inhabited succeeds if P is an inhabited typeclass and fails otherwise.
+*)
+Ltac tc_is_inhabited P :=
+  first [ let _ := constr:(ltac:(iSolveTC) : P) in idtac
+        | fail 1 "could not satisfy" P ].
+
+Ltac iDeex_one H :=
+  lazymatch iTypeOf H with
+  | Some (_, ?P) => lazymatch P with
+                    | named _ _ => idtac
+                    | _ => tc_is_inhabited (IsExistential P);
+                           iDestruct H as (?) H
+                    end
+  | None => fail 1 "iDeexHyp:" H "not found"
+  end.
+
+(* iDeexHyp is like [iDestruct "H" as (?) "H"] except that it preserves the name
+of the binder and repeats while the goal is an existential *)
+Ltac iDeexHyp H :=
+  iDeex_one H; repeat iDeex_one H.
+
+Lemma tac_name_replace {PROP:bi} (i: ident) Δ p (P: PROP) Q name :
+  envs_lookup i Δ = Some (p, named name P) →
+  match envs_simple_replace i p (Esnoc Enil (INamed name) P) Δ with
+  | Some Δ' => envs_entails Δ' Q
+  | None => False
+  end →
+  envs_entails Δ Q.
+Proof. rewrite /named. apply coq_tactics.tac_rename. Qed.
+
+Local Ltac iNameReplace i name :=
+  eapply (tac_name_replace i _ _ _ _ name);
+  [ first [ reduction.pm_reflexivity
+          | fail 1 "iNamed: could not find" i ]
+  | reduction.pm_reduce;
+    lazymatch goal with
+    | |- False => fail 1 "iNamed: name in not fresh" i
+    | _ => idtac
+    end
+  ].
+
+Lemma tac_name_intuitionistic {PROP:bi} Δ i i' p (P P' Q: PROP) name :
+  envs_lookup i Δ = Some (p, named name P) →
+  IntoPersistent p P P' →
+  (if p then TCTrue else TCOr (Affine P) (Absorbing Q)) →
+  match envs_replace i p true (Esnoc Enil i' P') Δ with
+  | Some Δ' => envs_entails Δ' Q
+  | None => False
+  end →
+  envs_entails Δ Q.
+Proof.
+  rewrite /named.
+  rewrite ?envs_entails_eq ?envs_entails_unseal => ? HP' HPQ HQ.
+  destruct (envs_replace _ _ _ _ _) as [Δ'|] eqn:Hrep; last done.
+  rewrite envs_replace_singleton_sound //.
+  rewrite HQ.
+
+  destruct p; simpl.
+  - iIntros "[#HP HQ]".
+    iApply "HQ".
+    iApply "HP".
+  - iIntros "[#HP HQ]".
+    iApply "HQ"; iFrame "#".
+Qed.
+
+Local Ltac iNameIntuitionistic i i' :=
+  eapply (tac_name_intuitionistic _ i i' _ _ _ _ _);
+  [ reduction.pm_reflexivity
+  | iSolveTC
+  | simpl; iSolveTC
+  | reduction.pm_reduce
+  ].
+
+Local Ltac iNamePure i name :=
+  let id := string_to_ident name in
+  let id := fresh id in
+  iPure i as id.
+
+(* iNameHyp implements naming a hypothesis of the form [H: name ∷ P].
+
+   The complete tactic is mutually recursive with iNamed_go for * patterns; this
+   self-contained version takes iNamed_go as a parameter *)
+Local Ltac iNameHyp_go_rx H iNamed_go :=
+  let i := to_pm_ident H in
+  lazymatch goal with
+  | |- context[Esnoc _ i (named ?name ?P)] =>
+    (* we check for some simple special-cases: *)
+    let pat := intro_pat.parse_one name in
+    lazymatch pat with
+    | IIdent (INamed ?name) =>
+      (* just rename one hypothesis *)
+      iNameReplace i name
+    | IIntuitionistic (IIdent ?i') =>
+      iNameIntuitionistic i i'
+    (* pure intros need to be freshened (otherwise they block using iNamed) *)
+    | IPure (IGallinaNamed ?name) =>
+      iNamePure i name
+    (* the token "*" causes iNamed to recurse *)
+    | IForall => change (Esnoc ?Δ i (named name P)) with (Esnoc Δ i P); iNamed_go i
+    | _ =>
+       (* we now do this only for backwards compatibility, which is a completely
+       safe but inefficient sequence that handles persistent/non-persistent
+       things correctly (most likely few patterns not covered above should even
+       be supported) *)
+       let Htmp := iFresh in
+       iRename i into Htmp;
+       iDestruct (from_named with Htmp) as pat;
+       try iClear Htmp
+    end
+  | |- context[Esnoc _ i _] =>
+    fail "iNameHyp: hypothesis" H "is not a named"
+  | _ => fail 1 "iNameHyp: hypothesis" H "not found"
+  end.
+
+(* The core of iNamed is destructing a spine of separating conjuncts and naming
+  each conjunct with iNameHyp; the implementation currently just calls iDestruct
+  and then attempts to name the new anonymous hypotheses, but it would be better
+  to parametrize the splitting and naming into a typeclass. *)
+Ltac iNamedDestruct_go_rx H iNameHyp :=
+  (* we track the original name H0 here so that at the very end we can name the
+  last conjunct if it isn't named (this is what PropRestore runs into - it can
+  be destructed until a final Restore hypothesis) *)
+  let rec go H0 H :=
+      first [ iNameHyp H
+            | lazymatch iTypeOf H with
+              | Some (_, ?P) => tc_is_inhabited (IsSplittable P)
+              | None => fail 1 "iNamed: hypothesis" H "not found"
+              end;
+              let Htmp1 := iFresh in
+              let Htmp2 := iFresh in
+              let pat := constr:(IList [[IIdent Htmp1; IIdent Htmp2]]) in
+              iDestruct H as pat;
+              iNameHyp Htmp1; go H0 Htmp2
+            | (* reaching here means the last conjunct could not be named with
+              iNameHyp; rather than leave it anonymous, restore the original
+              name (note this could fail if that name was used by one of the
+              inner names, which we don't handle here) *)
+              iRename H into H0 ] in
+  go H H.
+
+(* this declaration defines iNamed by tying together all the mutual recursion *)
+Local Ltac iNamed_go H :=
+  lazymatch H with
+  | 1%Z => let i := iFresh in iIntros i; iNamed_go i
+  | 1%nat => let i := iFresh in iIntros i; iNamed_go i
+  | _ =>
+    (* first destruct the existentials, then split the conjuncts (but
+    importantly only these two levels; the user must explicitly opt-in to
+    destructing more existentials for conjuncts) *)
+    try iDeexHyp H;
+    iNamedDestruct_go H
+  end with
+  (* Ltac *) iNameHyp_go H :=
+  iNameHyp_go_rx H iNamed_go with
+  (* Ltac *) iNamedDestruct_go H := iNamedDestruct_go_rx H iNameHyp_go.
+
+Tactic Notation "iNamedDestruct" constr(H) := iNamedDestruct_go H.
+Tactic Notation "iNamed" constr(H) := iNamed_go H.
+
+(* iNamed names any hypotheses that are anonymous but have a name. This is
+primarily useful when you for some reason need to introduce using ? and then
+separately name (this can arise if [iNamed] isn't doing the right thing, or
+wouldn't work for all the conjuncts) *)
+Tactic Notation "iNamed" :=
+  repeat match goal with
+         | |- context[Esnoc _ ?i (named ?name ?P)] =>
+           iNameHyp_go i
+         (* TODO: debug this for destructing anonymous composites *)
+         (* | |- context[Esnoc _ ?i ?P] =>
+           lazymatch P with
+           | context[named _ _] => progress iNamed i
+           end *)
+         end.
+
+(* iNameHyp only introduces names for a single hypothesis (and is usually not
+useful on its own) *)
+Ltac iNameHyp H := iNameHyp_go H.
+
+Tactic Notation "iNamedAccu" :=
+  iStartProof; eapply tac_named_accu; [ (* only one goal should spawn *)
+    first [
+        cbv [ env_to_named_prop env_to_named_prop_go ];
+        reduction.pm_reflexivity
+      | fail 1 "iNamedAccu: not an evar"
+      ]
+  ].
+
+Ltac iFrameNamed :=
+  lazymatch goal with
+  | [ |- envs_entails _ ?g ] =>
+    repeat match g with
+           | context[named ?p ?P] =>
+             let pat := intro_patterns.intro_pat.parse_one p in
+             lazymatch pat with
+             | IIdent ?name => iFrame name
+             | IIntuitionistic (IIdent ?name) => iFrame name
+             | IPure (IGallinaNamed ?name) =>
+               let name := string_to_ident name in
+               iFrame (name)
+             end
+           end
+  end.
+
+(* this is crucially placed just below level 80, which is where ∗ is, so that
+you can change [P ∗ Q] to ["HP" ∷ P ∗ "HQ" ∷ Q] without adding parentheses to
+attach the names correctly *)
+Notation "name ∷ P" := (named name P%I) (at level 79).
+
+(* Enable eauto to solve goals where the top-level is [named] *)
+Global Hint Extern 0 (environments.envs_entails _ (named _ _)) => unfold named : core.
+
+Ltac iSplitDelay :=
+  let PROP := iBiOfGoal in
+  let R := fresh "remainder" in
+  evar (R:PROP.(bi_car));
+  iApply (tac_delay_split R with "[-] []");
+  subst R.
